@prefix dqv:    <http://www.w3.org/ns/dqv#> .
@prefix xsd:    <http://www.w3.org/2001/XMLSchema#> .
@prefix rdfs:   <http://www.w3.org/2000/01/rdf-schema#> .
@prefix skos:   <http://www.w3.org/2004/02/skos/core#> .
@prefix dcat:   <http://www.w3.org/ns/dcat#> .
@prefix foaf:   <http://xmlns.com/foaf/0.1/> .
@prefix dct:    <http://purl.org/dc/terms/> .
@prefix cc:     <http://creativecommons.org/ns#> .
@prefix dcatno-mqa: <https://data.norge.no/vocabulary/dcatno-mqa#> .

# about this vocabulary

<https://data.norge.no/vocabulary/dcatno-mqa#>
   dct:title "Vokaublary for metadata quality assessment of the Norwegian data portal"@nb ;
   dct:description "This vocabulary specifies the metadata quality metrics for the Norwegian data portal data.norge.no."@en ;
   dct:modified "2022-04-12"^^xsd:date ;
   dct:format <http://publications.europa.eu/resource/authority/file-type/RDF_TURTLE> ;
   dct:creator [
        foaf:homepage <https://www.digdir.no/> ;
        foaf:name "Digitaliseringsdirektoratet"@nb ,
           "Norwegian Digitalisation Agency"@en ;
    ];
    cc:attributionURL <https://gitlab.com/dataeuropa/vocabularies/-/blob/master/piveau-dqv-vocabulary.ttl> ;
    dct:publisher <https://organization-catalog.data.norge.no/organizations/991825827> ;
   .

# Dimensions

dcatno-mqa:accessibility
    a                       dqv:Dimension ;
    skos:prefLabel          "Accessibility"@en ;
    skos:definition         "Once the user finds the required data, she/he needs to know how can they be accessed, possibly including authentication and authorisation."@en .

dcatno-mqa:contextuality
    a                       dqv:Dimension ;
    skos:prefLabel          "Contextuality"@en ;
    skos:definition         "Properties that provide more context for the user."@en .

dcatno-mqa:findability
    a                       dqv:Dimension ;
    skos:prefLabel          "Findability"@en ;
    skos:definition         "Metadata and data should be easy to find for both humans and computers. Machine-readable metadata are essential for automatic discovery of datasets and services."@en .

dcatno-mqa:interoperability
    a                       dqv:Dimension ;
    skos:prefLabel          "Interoperability"@en ;
    skos:definition         "Data usually needs to be integrated with other data. In addition, data needs to interoperate with applications or workflows for analysis, storage, and processing."@en .

dcatno-mqa:reusability
    a                       dqv:Dimension ;
    skos:prefLabel          "Reusability"@en ;
    skos:definition         "Metadata and data should be well-described so that they can be replicated and/or combined in different settings."@en .


# Five star

dcatno-mqa:OpenData5Star
    a                       skos:ConceptScheme;
    skos:prefLabel          "Open Data 5 Star"@en ;
    skos:definition         "Five star rating based on https://5stardata.info"@en ;
    dqv:inDimension         dcatno-mqa:interoperability .


dcatno-mqa:zeroStars
    a                       skos:Concept;
    skos:inScheme           dcatno-mqa:OpenData5Star ;
    skos:prefLabel          "Zero stars"@en ;
    skos:definition         "Dataset available on the web."@en .

dcatno-mqa:oneStar
    a                       skos:Concept;
    skos:inScheme           dcatno-mqa:OpenData5Star ;
    skos:prefLabel          "One star"@en ;
    skos:definition         "Dataset available on the web with open licence."@en .

dcatno-mqa:twoStars
    a                       skos:Concept;
    skos:inScheme           dcatno-mqa:OpenData5Star ;
    skos:prefLabel          "Two stars"@en ;
    skos:definition         "Dataset available on the web with open licence and structured, machine-readable format."@en .

dcatno-mqa:threeStars
    a                       skos:Concept;
    skos:inScheme           dcatno-mqa:OpenData5Star ;
    skos:prefLabel          "Three stars"@en ;
    skos:definition         "Dataset available on the web with open licence and structured, machine-readable, non proprietary format."@en .

dcatno-mqa:fourStars
    a                       skos:Concept;
    skos:inScheme           dcatno-mqa:OpenData5Star ;
    skos:prefLabel          "Four stars"@en ;
    skos:definition         "Dataset available on the web with open licence and structured, machine-readable, non proprietary format. It uses URIs to denote things."@en .

dcatno-mqa:fiveStars
    a                       skos:Concept;
    skos:inScheme           dcatno-mqa:OpenData5Star ;
    skos:prefLabel          "Five stars"@en ;
    skos:definition         "Dataset available on the web with open licence and structured, machine-readable, non proprietary format. It uses URIs to denote things and links to other resources for context."@en .


# Findability

dcatno-mqa:keywordAvailability
    a                       dqv:Metric ;
    skos:definition         "It is checked whether at least one dcat:keyword is specified in a dataset."@en ;
    dqv:expectedDataType    xsd:boolean ;
    dqv:inDimension         dcatno-mqa:findability .

dcatno-mqa:categoryAvailability
    a                       dqv:Metric ;
    skos:definition         "It is checked whether at least one dcat:theme is specified in a dataset."@en ;
    dqv:expectedDataType    xsd:boolean ;
    dqv:inDimension         dcatno-mqa:findability .

dcatno-mqa:spatialAvailability
    a                       dqv:Metric ;
    skos:definition         "It is checked whether at least one dct:spatial is specified in a dataset."@en ;
    dqv:expectedDataType    xsd:boolean ;
    dqv:inDimension         dcatno-mqa:findability .

dcatno-mqa:temporalAvailability
    a                       dqv:Metric ;
    skos:definition         "It is checked whether at least one dct:temporal is specified in a dataset."@en ;
    dqv:expectedDataType    xsd:boolean ;
    dqv:inDimension         dcatno-mqa:findability .



# Accessibility

dcatno-mqa:accessUrlStatusCode
    a                       dqv:Metric ;
    skos:definition         "A distribution's dcat:accessURL is checked for accessibility via HTTP HEAD request. The response contains a numeric status code."@en ;
    dqv:expectedDataType    xsd:integer ;
    dqv:inDimension         dcatno-mqa:accessibility .

dcatno-mqa:downloadUrlAvailability
    a                       dqv:Metric ;
    skos:definition         "It is checked whether at least one dcat:downloadUrl is specified in a distribution."@en ;
    dqv:expectedDataType    xsd:boolean ;
    dqv:inDimension         dcatno-mqa:accessibility .

dcatno-mqa:downloadUrlStatusCode
    a                       dqv:Metric ;
    skos:definition         "A distribution's dcat:downloadURL is checked for accessibility via HTTP HEAD request. The response contains a numeric status code."@en ;
    dqv:expectedDataType    xsd:integer ;
    dqv:inDimension         dcatno-mqa:accessibility .



# Interoperability

dcatno-mqa:formatAvailability
    a                       dqv:Metric ;
    skos:definition         "It is checked whether dct:format is specified in a distribution."@en ;
    dqv:expectedDataType    xsd:boolean ;
    dqv:inDimension         dcatno-mqa:interoperability .

dcatno-mqa:mediaTypeAvailability
    a                       dqv:Metric ;
    skos:definition         "It is checked whether dcat:mediaType is specified in a distribution."@en ;
    dqv:expectedDataType    xsd:boolean ;
    dqv:inDimension         dcatno-mqa:interoperability .

dcatno-mqa:formatMediaTypeVocabularyAlignment
    a                       dqv:Metric ;
    skos:definition         "Checks if both a distribution&apos;s dct:format and dcat:mediaType are aligned to the  controlled vocabulary specified by DCAT-AP."@en ;
    dqv:expectedDataType    xsd:boolean ;
    dqv:inDimension         dcatno-mqa:interoperability .

dcatno-mqa:formatMediaTypeNonProprietary
    a                       dqv:Metric ;
    skos:definition         "Checks if at least one of a distribution&apos;s dct:format and dcat:mediaType is non-proprietary. If neither is set it is assumed the distribution uses a proprietary format/media type."@en ;
    dqv:expectedDataType    xsd:boolean ;
    dqv:inDimension         dcatno-mqa:interoperability .

dcatno-mqa:formatMediaTypeMachineInterpretable
    a                       dqv:Metric ;
    skos:definition         "Checks if at least one of a distribution's dct:format and dcat:mediaType is machine-interpretable. If neither is set it is assumed the distribution uses a non-machine-interpretable format/media type."@en ;
    dqv:expectedDataType    xsd:boolean ;
    dqv:inDimension         dcatno-mqa:interoperability .

dcatno-mqa:dcatApCompliance
    a                       dqv:Metric ;
    skos:definition         "A dataset is validated for conformity against the DCAT-AP specification using SHACL rules."@en ;
    dqv:expectedDataType    xsd:boolean ;
    dqv:inDimension         dcatno-mqa:interoperability .

dcatno-mqa:formatMatch
    a                       dqv:Metric ;
    skos:definition         "It is checked whether a distributions's dct:format property resembles the actual format of the linked file."@en ;
    dqv:expectedDataType    xsd:boolean ;
    dqv:inDimension         dcatno-mqa:interoperability .

dcatno-mqa:syntaxValid
    a                       dqv:Metric ;
    skos:definition         "It is checker whether a file's content is syntactically valid against the format's specification."@en ;
    dqv:expectedDataType    xsd:boolean ;
    dqv:inDimension         dcatno-mqa:interoperability .

dcatno-mqa:atLeastFourStars
    a                       dqv:Metric ;
    skos:definition         "Checks if the dataset got at least a four stars rating." ;
    dqv:expectedDataType    xsd:boolean ;
    dqv:inDimension         dcatno-mqa:interoperability .


# Reusability

dcatno-mqa:licenceAvailability
    a                       dqv:Metric ;
    skos:definition         "It is checked whether dct:license is specified in a distribution."@en ;
    dqv:expectedDataType    xsd:boolean ;
    dqv:inDimension         dcatno-mqa:reusability .

dcatno-mqa:knownLicence
    a                       dqv:Metric ;
    skos:definition         "It is checked if a distribution&apos;s licence is part of a predefined collection."@en ;
    dqv:expectedDataType    xsd:boolean ;
    dqv:inDimension         dcatno-mqa:reusability .

dcatno-mqa:accessRightsAvailability
    a                       dqv:Metric ;
    skos:definition         "It is checked whether dct:accessRights is specified in a dataset."@en ;
    dqv:expectedDataType    xsd:boolean ;
    dqv:inDimension         dcatno-mqa:reusability .

dcatno-mqa:accessRightsVocabularyAlignment
    a                       dqv:Metric ;
    skos:definition         "Checks if a dataset&apos;s dct:accessRights is aligned to the controlled vocabulary specified by DCAT-AP."@en ;
    dqv:expectedDataType    xsd:boolean ;
    dqv:inDimension         dcatno-mqa:reusability .

dcatno-mqa:contactPointAvailability
    a                       dqv:Metric ;
    skos:definition         "It is checked whether dcat:contactPoint is specified in a dataset."@en ;
    dqv:expectedDataType    xsd:boolean ;
    dqv:inDimension         dcatno-mqa:reusability .

dcatno-mqa:publisherAvailability
    a                       dqv:Metric ;
    skos:definition         "It is checked whether a dct:publisher is specified in a dataset."@en ;
    dqv:expectedDataType    xsd:boolean ;
    dqv:inDimension         dcatno-mqa:reusability .

dcatno-mqa:openLicense # Norwegian extension
    a                       dqv:Metric ;
    skos:definition         "It is checked if a distribution&apos;s licence is an open-source license."@en ;
    dqv:expectedDataType    xsd:boolean ;
    dqv:inDimension         dcatno-mqa:reusability .


# Contextuality

dcatno-mqa:rightsAvailability
    a                       dqv:Metric ;
    skos:definition         "It is checked whether dct:rights is specified in a distribution."@en ;
    dqv:expectedDataType    xsd:boolean ;
    dqv:inDimension         dcatno-mqa:contextuality .

dcatno-mqa:byteSizeAvailability
    a                       dqv:Metric ;
    skos:definition         "It is checked whether dcat:byteSize is specified in a distribution."@en ;
    dqv:expectedDataType    xsd:boolean ;
    dqv:inDimension         dcatno-mqa:contextuality .

dcatno-mqa:dateIssuedAvailability
    a                       dqv:Metric ;
    skos:definition         "It is checked whether dct:issued is specified in a distribution."@en ;
    dqv:expectedDataType    xsd:boolean ;
    dqv:inDimension         dcatno-mqa:contextuality .

dcatno-mqa:dateModifiedAvailability
    a                       dqv:Metric ;
    skos:definition         "It is checked whether dct:modified is specified in a distribution."@en ;
    dqv:expectedDataType    xsd:boolean ;
    dqv:inDimension         dcatno-mqa:contextuality .

dcatno-mqa:score
    a                       dqv:Metric ;
    skos:definition         "It is calculated a score from the measurements results based on the corresponding score values."@en ;
    dqv:expectedDataType    xsd:integer ;
    dqv:inDimension         dcatno-mqa:contextuality .


# additional properties

dcatno-mqa:trueScore
    a                       rdfs:Property .

dcatno-mqa:falseScore
    a                       rdfs:Property .
